feat: add combinators for more fine-grained benchmarking (#198)
### Description:

This adds combinators to benchmark specific parts of a tactic, either by
directly outputting the data, or by storing datapoints in a state for
aggregation. Either behaviour is controlled by a `benchmark` option,
which defaults to false, but is set to `true` in the benchmark command.

### Testing:

What tests have been run? Did `make all` succeed for your changes? Was
conformance testing successful on an Aarch64 machine? yes

### License:

By submitting this pull request, I confirm that my contribution is
made under the terms of the Apache 2.0 license.

---------

Co-authored-by: Shilpi Goel <shigoel@gmail.com>

Benchmarks/Command.lean
@@ -7,21 +7,38 @@ import Lean
 
 open Lean Parser.Command Elab.Command
 
+initialize
+  registerOption `benchmark {
+    defValue := false
+    descr := "enables/disables benchmarking in `withBenchmark` combinator"
+  }
+
+variable {m} [Monad m] [MonadLiftT BaseIO m] in
+def withHeartbeatsAndMs (x : m α) : m (α × Nat × Nat) := do
+  let start ← IO.monoMsNow
+  let (a, heartbeats) ← withHeartbeats x
+  let endTime ← IO.monoMsNow
+  return ⟨a, heartbeats, endTime - start⟩
+
 elab "benchmark" id:ident declSig:optDeclSig val:declVal : command => do
-  let stx ← `(command| example $declSig:optDeclSig $val:declVal )
+  logInfo m!"Running {id} benchmark\n"
+
+  let stx ← `(command|
+    set_option benchmark true in
+    example $declSig:optDeclSig $val:declVal
+  )
 
   let n := 5
-  let mut runTimes := #[]
   let mut totalRunTime := 0
-  -- geomean = exp(log((a₁ a₂ ... aₙ)^1/n)) = 
+  -- geomean = exp(log((a₁ a₂ ... aₙ)^1/n)) =
   -- exp(1/n * (log a₁ + log a₂ + log aₙ)).
   let mut totalRunTimeLog := 0
-  for _ in [0:n] do
-    let start ← IO.monoMsNow
-    elabCommand stx
-    let endTime ← IO.monoMsNow
-    let runTime := endTime - start
-    runTimes := runTimes.push runTime
+  for i in [0:n] do
+    logInfo m!"\n\nRun {i} (out of {n}):\n"
+    let ((), _, runTime) ← withHeartbeatsAndMs <|
+      elabCommand stx
+
+    logInfo m!"Proof took {runTime / 1000}s in total"
     totalRunTime := totalRunTime + runTime
     totalRunTimeLog := totalRunTimeLog + Float.log runTime.toFloat
 
@@ -33,22 +50,158 @@ elab "benchmark" id:ident declSig:optDeclSig val:declVal : command => do
     {avg}s
   geomean over {n} runs:
     {geomean}s
-
-  indidividual runtimes:
-    {runTimes}
 "
+
+/-- Set various options to disable linters -/
+macro "disable_linters" "in" cmd:command : command => `(command|
+  set_option linter.constructorNameAsVariable false in
+  set_option linter.deprecated false in
+  set_option linter.missingDocs false in
+  set_option linter.omit false in
+  set_option linter.suspiciousUnexpanderPatterns false in
+  set_option linter.unnecessarySimpa false in
+  set_option linter.unusedRCasesPattern false in
+  set_option linter.unusedSectionVars false in
+  set_option linter.unusedVariables false in
+  $cmd
+)
 
 /-- The default `maxHeartbeats` setting.
 
 NOTE: even if the actual default value changes at some point in the future,
 this value should *NOT* be updated, to ensure the percentages we've reported
 in previous versions remain comparable. -/
-def defaultMaxHeartbeats : Nat := 200000
+private def defaultMaxHeartbeats : Nat := 200000
+
+private def percentOfDefaultMaxHeartbeats (heartbeats : Nat) : Nat :=
+  heartbeats / (defaultMaxHeartbeats * 10)
 
 open Elab.Tactic in
 elab "logHeartbeats" tac:tactic : tactic => do
   let ((), heartbeats) ← withHeartbeats <|
     evalTactic tac
-  let percent := heartbeats / (defaultMaxHeartbeats * 10)
+  let percent := percentOfDefaultMaxHeartbeats heartbeats
 
   logInfo m!"used {heartbeats / 1000} heartbeats ({percent}% of the default maximum)"
+
+section withBenchmark
+variable {m} [Monad m] [MonadLiftT BaseIO m] [MonadOptions m] [MonadLog m]
+  [AddMessageContext m]
+
+/-- if the `benchmark` option is true, execute `x` and call `f` with the amount
+of heartbeats and milliseconds (in that order!) taken by `x`.
+
+Otherwise, just execute `x` without measurements. -/
+private def withBenchmarkAux (x : m α) (f : Nat → Nat → m Unit)  : m α := do
+  if (← getBoolOption `benchmark) = false then
+    x
+  else
+    let (a, heartbeats, t) ← withHeartbeatsAndMs x
+    f heartbeats t
+    return a
+
+
+/-- `withBenchmark header x` is a combinator that will, if the `benchmark`
+option is set to `true`, log the time and heartbeats used by `x`,
+in a message like:
+  `{header} took {x}s and {y} heartbeats ({z}% of the default maximum)`
+
+Otherwise, if `benchmark` is set to false, `x` is returned as-is.
+
+NOTE: the maximum reffered to in the message is `defaultMaxHeartbeats`,
+deliberately *not* the currently confiugred `maxHeartbeats` option, to keep the
+numbers comparable across different values of that option. It's thus entirely
+possible to see more than 100% being reported here. -/
+def withBenchmark (header : String) (x : m α) : m α := do
+  withBenchmarkAux x fun heartbeats t => do
+    let percent := percentOfDefaultMaxHeartbeats heartbeats
+    logInfo m!"{header} took: {t}ms and {heartbeats} heartbeats \
+      ({percent}% of the default maximum)"
+
+/-- Benchmark the time and heartbeats taken by a tactic, if the `benchmark`
+option is set to `true` -/
+elab "with_benchmark" t:tactic : tactic => do
+  withBenchmark "{t}" <| Elab.Tactic.evalTactic t
+
+end withBenchmark
+
+/-!
+## Aggregated benchmark statistics
+We define `withAggregatedBenchmark`, which functions like `withBenchmark`,
+except it will store a running average of the statistics in a `BenchmarkState`
+which will be reported in one go when `reportAggregatedBenchmarks` is called.
+-/
+section
+
+structure BenchmarkState.Stats where
+  totalHeartbeats : Nat := 0
+  totalTimeInMs : Nat := 0
+  samples : Nat := 0
+
+structure BenchmarkState where
+  insertionOrder : List String := []
+  stats : Std.HashMap String BenchmarkState.Stats := .empty
+
+variable {m} [Monad m] [MonadStateOf BenchmarkState m] [MonadLiftT BaseIO m]
+  [MonadOptions m]
+
+/-- `withAggregatedBenchmark header x` is a combinator that will,
+if the `benchmark` option is set to `true`,
+measure the time and heartbeats to the benchmark state in a way that aggregates
+different measurements with the same `header`.
+
+See `reportAggregatedBenchmarks` to log the collected data.
+
+Otherwise, if `benchmark` is set to false, `x` is returned as-is.
+-/
+def withAggregatedBenchmark (header : String) (x : m α) : m α := do
+  withBenchmarkAux x fun heartbeats t => do
+    modify fun state =>
+      let s := state.stats.getD header {}
+      { insertionOrder :=
+          if s.samples = 0 then
+            header :: state.insertionOrder
+          else
+            state.insertionOrder
+        stats := state.stats.insert header {
+          totalHeartbeats := s.totalHeartbeats + heartbeats
+          totalTimeInMs   := s.totalTimeInMs + t
+          samples         := s.samples + 1
+      }}
+
+variable [MonadLog m] [AddMessageContext m] in
+/--
+if the `benchmark` option is set to `true`, report the data collected by
+`withAggregatedBenchmark`, and reset the state (so that the next call to
+`reportAggregatedBenchmarks` will report only new data).
+-/
+def reportAggregatedBenchmarks : m Unit := do
+  if (← getBoolOption `benchmark) = false then
+    return
+
+  let { insertionOrder, stats } ← get
+  for header in insertionOrder do
+    let stats := stats.getD header {}
+    let heartbeats := stats.totalHeartbeats
+    let percent := percentOfDefaultMaxHeartbeats heartbeats
+    let t := stats.totalTimeInMs
+    let n := stats.samples
+    logInfo m!"{header} took: {t}ms and {heartbeats} heartbeats \
+      ({percent}% of the default maximum) in total over {n} samples"
+
+  set ({} : BenchmarkState)
+
+abbrev BenchT := StateT BenchmarkState
+
+variable [MonadLog m] [AddMessageContext m] in
+/--
+Execute `x` with the default `BenchmarkState`, and report the benchmarks after
+(see `reportAggregatedBenchmarks`).
+-/
+def withBenchmarksReport (x : BenchT m α) : m α :=
+  (Prod.fst <$> ·) <| StateT.run (s := {}) do
+    let a ← x
+    reportAggregatedBenchmarks
+    return a
+
+end
